aneris/examples/transactional_consistency/read_committed/implication_proof/si_implies_rc.v
@@ -42,6 +42,7 @@ Section Implication.
       KVS_Init := SI.(snapshot_isolation.specs.resources.KVS_Init);
       KVS_ClientCanConnect sa := SI.(snapshot_isolation.specs.resources.KVS_ClientCanConnect) sa;
       Seen k V := (∃ h, ⌜∀ v, v ∈ V → v ∈ h⌝ ∗ SI.(snapshot_isolation.specs.resources.Seen) k h)%I;
+      extract c := SI.(snapshot_isolation.specs.resources.extract) c;
     |}.
   Next Obligation.
     iIntros (SI k cst v) "[[%V [%h (%Hfalse & _)]] | (%Hneq & Hupd & Hkey)]"; first done. 
@@ -81,15 +82,15 @@ Section Implication.
       by destruct (Himp v) as [_ Hgoal].
   Qed.
   Next Obligation.
-    iIntros (SI E c c' sa sa' ls ls' Hsub) 
-      "#Hinv ([(-> & Hconn1) | [%m (-> & Hconn1)]] & [(-> & Hconn2) | [%m' (-> & Hconn2)]])".
-    all : iMod (SI.(snapshot_isolation.specs.resources.Connection_unique) 
-            with "[$Hinv][$Hconn1 $Hconn2]") as "(Hconn1 & Hconn2 & Heq)"; first done.
-    all : iModIntro.
-    all : iFrame.
-    all : iSplitL "Hconn1".
-    1, 2, 3, 6 : iLeft; by iFrame.
-    1, 2, 3, 4 : iRight; iExists _; by iFrame.
+    simpl.
+    iIntros (SI sa c) "Hconn".
+    iApply (SI.(snapshot_isolation.specs.resources.Extraction_of_address) 
+      with "[$Hconn]").
+  Qed.
+  Next Obligation.
+    simpl.
+    iIntros (SI sa sa' c c' Heq1 Heq2 Hneq).
+    by eapply SI.(snapshot_isolation.specs.resources.Extraction_preservation).
   Qed.
 
   Lemma rewrite_maps_1 `{SI : !SI_resources Mdl Σ} (m : gmap Key Vals) :
